src/HOL/CVC/cvc5_dsl_rewrites/BV_Rewrites_Elimination.thy
@@ -2,6 +2,9 @@ theory BV_Rewrites_Elimination
   imports BV_Rewrites_Lemmas 
 begin
 
+declare[[show_types,show_sorts]]
+declare[[smt_expert_debug_alethe_level=0]]
+
 (*
 (define-rule bv-ugt-eliminate
   ((x ?BitVec) (y ?BitVec))
@@ -83,6 +86,36 @@ lemma [rewrite_bv_slt_eliminate]:
   by (metis add.commute add_lessD1 n_less_equal_power_2 nat_int of_nat_take_bit plus_1_eq_Suc take_bit_nat_eq_self)
 
 (*
+(define-cond-rule bv-redor-eliminate
+  ((x ?BitVec) (w Int))
+  (= w (@bvsize x))
+  (bvredor x)
+  (bvnot (bvcomp x (@bv 0 w))))
+*)
+
+named_theorems rewrite_bv_redor_eliminate \<open>automatically_generated\<close>
+
+lemma [rewrite_bv_redor_eliminate]:
+  fixes x::"'a ::len word"
+  shows "smt_redor x = not (smt_comp x (Word.Word (0::int)))"
+  unfolding smt_redor_def by simp
+
+(*
+(define-cond-rule bv-redand-eliminate
+  ((x ?BitVec) (w Int))
+  (= w (@bvsize x))
+  (bvredand x)
+  (bvcomp x (bvnot (@bv 0 w))))
+*)
+
+named_theorems rewrite_bv_redand_eliminate \<open>automatically_generated\<close>
+
+lemma [rewrite_bv_redand_eliminate]:
+  fixes x::"'a ::len word"
+  shows "smt_redand x = smt_comp x (not (Word.Word (0::int)))"
+  unfolding smt_redand_def by auto
+
+(*
 (define-rule bv-ule-eliminate
   ((x ?BitVec) (y ?BitVec))
   (bvule x y)
@@ -96,6 +129,355 @@ lemma [rewrite_bv_ule_eliminate]:
     \<Longrightarrow> (x \<le> y) = (\<not>(y < x))"
   using word_le_not_less by simp
 
+(*
+(define-rule bv-comp-eliminate
+  ((x ?BitVec) (y ?BitVec))
+  (bvcomp x y)
+  (ite (= x y) (@bv 1 1) (@bv 0 1)))
+*)
+
+named_theorems rewrite_bv_comp_eliminate \<open>automatically_generated\<close>
+
+lemma [rewrite_bv_comp_eliminate]:
+  fixes x::"'a ::len word" and y::"'a ::len word"
+  shows "smt_comp x y = (if x = y then Word.Word (1::int) else Word.Word (0::int))"
+  by (metis one_word.abs_eq smt_comp_def zero_word.abs_eq)
 
 
+(*
+(define-cond-rule bv-rotate-left-eliminate-1
+  ((x ?BitVec) (amount Int) (u1 Int) (u2 Int) (l2 Int))
+  (def (n (@bvsize x)) (a (mod amount n)))
+  (and (not (= a 0)) (= u1 (- n (+ 1 a))) (= u2 (- n 1)) (= l2 (- n a)))
+  (rotate_left amount x)
+  (concat
+    (extract u1 0 x)
+    (extract u2 l2 x)))
+*)
+
+
+named_theorems rewrite_bv_rotate_left_eliminate_1 \<open>automatically_generated\<close>
+
+(*lemma is somehow wrong*)
+(*
+lemma [rewrite_bv_rotate_left_eliminate_1]:
+  fixes x::"'a::len word" and amount::"int"
+  assumes "SMT.z3mod amount (int (size x)) \<noteq> (0::int)"
+    "size x - (1 + SMT.z3mod amount (int (size x))) \<ge> 0"
+    "size x - (1 + SMT.z3mod amount (int (size x))) < LENGTH('a)"
+    "LENGTH('b) = size x - (1 + SMT.z3mod amount (int (size x))) + 1"
+    "size x - SMT.z3mod amount (int (size x)) \<ge> 0"
+    "size x - SMT.z3mod amount (int (size x)) \<le> size x -1"
+    "size x - 1 < LENGTH('a)"
+    "LENGTH('c) = SMT.z3mod amount (int (size x))"
+    "LENGTH('a) = LENGTH('b) + LENGTH('c)"
+    "amount \<ge> 0"
+  shows "
+  (word_rotl (nat amount) x::'a::len word) =
+   word_cat
+    (smt_extract
+      (nat (int (size x) - ((1::int) + SMT.z3mod amount (int (size x)))))
+      (nat (0::int)) x::'b::len word)
+    (smt_extract (nat (int (size x) - (1::int)))
+      (nat (int (size x) - SMT.z3mod amount (int (size x)))) x::'c::len word)"
+proof -
+  let ?n = "LENGTH('a)"
+  define a where "a = LENGTH('c)"
+
+  have size_eq: "size x = ?n" by (simp add: word_size)
+
+  have z3mod_nneg: "0 \<le> SMT.z3mod amount (int (size x))"
+    by (simp add: SMT.z3mod_def)
+
+  have t0: "(0 \<le> amount mod (int LENGTH('b) + SMT.z3mod amount (int (size x))))"
+    using  a_def assms(9) len_num1 n_not_Suc_n plus_1_eq_Suc
+    unfolding SMT.z3mod_def 
+    by (simp add: assms(10) nonneg_mod_div)
+    
+  text \<open>The rotation amount, reduced modulo \<open>?n\<close>, equals \<open>LENGTH('c)\<close>.\<close>
+  have shift_mod: "nat amount mod (LENGTH('b) + LENGTH('c)) = LENGTH('c)"
+    apply (simp add: nat_mod_as_int)
+    apply (subst int_int_eq[symmetric])
+    apply (subst assms(8))
+    apply (subst assms(10))
+    apply simp
+    apply (simp add: t0)
+    apply (simp add: assms(10))
+    unfolding SMT.z3mod_def sorry
+  have shift_eq: "nat amount mod ?n = a"
+    using shift_mod assms(9) a_def by simp
+
+  have b_eq: "LENGTH('b) = ?n - a"
+    using assms(9) a_def by simp
+  have a_lt_n: "a < ?n"
+    using shift_eq[symmetric] by simp
+
+  have z3mod_nat: "nat (SMT.z3mod amount (int (size x))) = a"
+    using assms(10) size_eq shift_eq
+    by (simp add: SMT.z3mod_def nat_mod_distrib flip: zmod_int)
+
+  have a_pos: "0 < a"
+    using assms(1) z3mod_nneg z3mod_nat by (metis nat_0 order_le_imp_less_or_eq)
+
+  text \<open>Rewrite the integer-shaped indices in \<open>nat\<close> arithmetic.\<close>
+  have idx_hi: "nat (int (size x) - (1 + SMT.z3mod amount (int (size x)))) = ?n - 1 - a"
+    using z3mod_nat z3mod_nneg size_eq assms(2)
+    by (simp add: nat_diff_distrib nat_add_distrib)
+  have idx_top: "nat (int (size x) - 1) = ?n - 1"
+    using size_eq by (simp add: nat_diff_distrib)
+  have idx_lo: "nat (int (size x) - SMT.z3mod amount (int (size x))) = ?n - a"
+    using z3mod_nat z3mod_nneg size_eq assms(5)
+    by (simp add: nat_diff_distrib)
+
+  show ?thesis
+    unfolding idx_hi idx_top idx_lo
+  proof (rule bit_word_eqI)
+    fix k :: nat
+    assume k_lt: "k < ?n"
+    show "bit (word_rotl (nat amount) x) k =
+          bit (word_cat
+                 (smt_extract (?n - 1 - a) (nat 0) x :: 'b word)
+                 (smt_extract (?n - 1) (?n - a) x :: 'c word) :: 'a word) k"
+    proof (cases "k < a")
+      case True
+      with a_lt_n have add_lt: "k + (?n - a) < ?n" by linarith
+      have lhs: "bit (word_rotl (nat amount) x) k = bit x (k + (?n - a))"
+        using k_lt shift_eq add_lt by (simp add: bit_word_rotl_iff)
+      have rhs: "bit (word_cat
+                       (smt_extract (?n - 1 - a) (nat 0) x :: 'b word)
+                       (smt_extract (?n - 1) (?n - a) x :: 'c word) :: 'a word) k
+                  = bit x (k + (?n - a))"
+        using True k_lt a_lt_n a_pos b_eq a_def add_lt
+        by (auto simp: bit_word_cat_iff bit_smt_extract)
+      from lhs rhs show ?thesis by simp
+    next
+      case False
+      then have k_ge: "a \<le> k" by simp
+      with k_lt a_lt_n have k_minus_lt: "k - a < ?n - a" by linarith
+      have add_eq: "(k + (?n - a)) mod ?n = k - a"
+      proof -
+        have "k + (?n - a) = (k - a) + ?n"
+          using k_ge a_lt_n by simp
+        then show ?thesis using k_minus_lt by simp
+      qed
+      have lhs: "bit (word_rotl (nat amount) x) k = bit x (k - a)"
+        using k_lt shift_eq add_eq by (simp add: bit_word_rotl_iff)
+      have rhs: "bit (word_cat
+                       (smt_extract (?n - 1 - a) (nat 0) x :: 'b word)
+                       (smt_extract (?n - 1) (?n - a) x :: 'c word) :: 'a word) k
+                  = bit x (k - a)"
+        using False k_lt a_lt_n a_pos b_eq a_def k_minus_lt k_ge
+        by (auto simp: bit_word_cat_iff bit_smt_extract)
+      from lhs rhs show ?thesis by simp
+    qed
+  qed
+qed
+*)
+
+(*
+(define-cond-rule bv-rotate-left-eliminate-2
+  ((x ?BitVec) (amount Int))
+  (= (mod amount (@bvsize x)) 0)
+  (rotate_left amount x)
+  x)
+*)
+
+
+named_theorems rewrite_bv_rotate_left_eliminate_2 \<open>automatically_generated\<close>
+
+lemma [rewrite_bv_rotate_left_eliminate_2]:
+  fixes x::"'a::len word" and amount::"int"
+  shows "SMT.z3mod amount (int (size x)) = (0::int) \<longrightarrow>
+   word_rotl (nat amount) x = x"
+  unfolding SMT.z3mod_def
+  apply (simp only: word_uint_eq_iff)
+  apply (simp add: uint_word_rotl_eq)
+  apply (simp add: unsigned_take_bit_eq)
+  unfolding concat_bit_def
+  by (simp add: bintr_uint nat_mod_as_int size_word.rep_eq)
+
+
+(*
+(define-cond-rule bv-rotate-right-eliminate-1
+  ((x ?BitVec) (amount Int) (u1 Int) (u2 Int) (l2 Int))
+  (def (n (@bvsize x)) (a (mod amount n)))
+  (and (not (= a 0)) (= u1 (- a 1)) (= u2 (- n 1)) (= l2 a))
+  (rotate_right amount x)
+  (concat
+    (extract u1 0 x)
+    (extract u2 l2 x)))
+*)
+
+named_theorems rewrite_bv_rotate_right_eliminate_1 \<open>automatically_generated\<close>
+
+lemma [rewrite_bv_rotate_right_eliminate_1]:
+  fixes x::"'a::len word" and amount::"int"
+  shows "SMT.z3mod amount (int (size x)) \<noteq> (0::int) \<longrightarrow>
+  LENGTH('a) = LENGTH('b) + LENGTH('c) \<longrightarrow>
+  amount \<ge> 0 \<longrightarrow> 
+  SMT.z3mod amount (int (size x)) - 1 \<ge> 0 \<longrightarrow>
+  SMT.z3mod amount (int (size x)) - 1 < LENGTH('a) \<longrightarrow>
+  LENGTH('b) = SMT.z3mod amount (int (size x)) \<longrightarrow>
+  SMT.z3mod amount (int (size x)) \<ge> 0 \<longrightarrow>
+  size x - 1 \<ge> SMT.z3mod amount (int (size x)) \<longrightarrow> 
+  size x - 1 \<le> LENGTH('a) \<longrightarrow>
+  LENGTH('c) = size x - SMT.z3mod amount (int (size x)) \<longrightarrow>
+  (word_rotr (nat amount) x::'a::len word) =
+   word_cat
+    (smt_extract (nat (SMT.z3mod amount (int (size x)) - (1::int)))
+      (nat (0::int)) x::'b::len word)
+    (smt_extract (nat (int (size x) - (1::int)))
+      (nat (SMT.z3mod amount (int (size x)))) x::'c::len word)"
+(*  apply (rule impI)+
+  apply (simp only: word_uint_eq_iff )
+    apply (simp add: uint_word_rotr_eq)
+  apply (simp add: concat_bit_eq uint_take_bit_eq)
+  apply (subst uint_word_cat[of "(smt_extract (nat (SMT.z3mod amount (int (size x)) - (1::int)))
+      0 x::'b::len word)" "(smt_extract (nat (int (size x) - (1::int)))
+      (nat (SMT.z3mod amount (int (size x)))) x::'c::len word)", where 'c="'a"])
+   apply simp
+  apply (subst uint_smt_extract[of 0 "(nat (SMT.z3mod amount (int (size x)) - (1::int)))" x, where 'b="'b"])
+     apply simp_all
+  apply (subst uint_smt_extract[of "(nat (SMT.z3mod amount (int (size x))))" "(nat (int (size x) - (1::int)))" x, where 'b="'c"])
+  apply simp_all
+    apply (simp add: push_bit_take_bit)
+  apply (simp add: drop_bit_take_bit)
+  using Suc_diff_1
+  unfolding SMT.z3mod_def
+  apply (simp add:  nat_mod_as_int)*)
+ (* by (smt (verit, ccfv_SIG) Suc_nat_eq_nat_zadd1 add.right_neutral diff_add_inverse group_cancel.add2 int_nat_eq nat_int plus_1_eq_Suc size_word.rep_eq zmod_int)
+*)
+  sorry
+(*
+(define-cond-rule bv-rotate-right-eliminate-2
+  ((x ?BitVec) (amount Int))
+  (= (mod amount (@bvsize x)) 0)
+  (rotate_right amount x)
+  x)
+
+(define-rule bv-nand-eliminate
+  ((x ?BitVec) (y ?BitVec))
+  (bvnand x y)
+  (bvnot (bvand x y)))
+(define-rule bv-nor-eliminate
+  ((x ?BitVec) (y ?BitVec))
+  (bvnor x y)
+  (bvnot (bvor x y)))
+(define-rule bv-xnor-eliminate
+  ((x ?BitVec) (y ?BitVec))
+  (bvxnor x y)
+  (bvnot (bvxor x y)))
+
+(define-cond-rule bv-sdiv-eliminate
+  ((x ?BitVec) (y ?BitVec) (nm1 Int))
+  (def
+    (xLt0 (= (extract nm1 nm1 x) (@bv 1 1)))
+    (yLt0 (= (extract nm1 nm1 y) (@bv 1 1)))
+    (rUdiv (bvudiv (ite xLt0 (bvneg x) x) (ite yLt0 (bvneg y) y)))
+  )
+  (= nm1 (- (@bvsize x) 1))
+  (bvsdiv x y)
+  (ite (xor xLt0 yLt0) (bvneg rUdiv) rUdiv))
+
+(define-rule bv-zero-extend-eliminate
+  ((x ?BitVec) (n Int))
+  (zero_extend n x)
+  (concat (@bv 0 n) x))
+
+(define-cond-rule bv-uaddo-eliminate
+  ((x ?BitVec) (y ?BitVec) (w Int))
+  (= w (@bvsize x))
+  (bvuaddo x y)
+  (= (extract w w
+      (bvadd (concat (@bv 0 1) x) (concat (@bv 0 1) y)))
+    (@bv 1 1)
+  ))
+(define-cond-rule bv-saddo-eliminate
+  ((x ?BitVec) (y ?BitVec) (wm1 Int))
+  (def
+    (xS (extract wm1 wm1 x))
+    (yS (extract wm1 wm1 y))
+    (aS (extract wm1 wm1 (bvadd x y)))
+  )
+  (= wm1 (- (@bvsize x) 1))
+  (bvsaddo x y)
+  (or
+    (and (and (= xS (@bv 1 1)) (= yS (@bv 1 1))) (= aS (@bv 0 1)))
+    (and (and (= xS (@bv 0 1)) (= yS (@bv 0 1))) (= aS (@bv 1 1)))
+  ))
+(define-cond-rule bv-sdivo-eliminate
+  ((x ?BitVec) (y ?BitVec) (w Int) (wm1 Int))
+  (and (= wm1 (- (@bvsize x) 1)) (= w (@bvsize y)))
+  (bvsdivo x y)
+  (and
+    (= x (concat (@bv 1 1) (@bv 0 wm1)))
+    (= y (bvnot (@bv 0 w)))
+  ))
+(define-cond-rule bv-smod-eliminate
+  ((x ?BitVec) (y ?BitVec) (w Int) (wm1 Int))
+  (def
+    (xLt0 (= (extract wm1 wm1 x) (@bv 1 1)))
+    (yLt0 (= (extract wm1 wm1 y) (@bv 1 1)))
+    (nxLt0 (= (extract wm1 wm1 x) (@bv 0 1)))
+    (nyLt0 (= (extract wm1 wm1 y) (@bv 0 1)))
+    (xAbs (ite nxLt0 x (bvneg x)))
+    (yAbs (ite nyLt0 y (bvneg y)))
+    (u (bvurem xAbs yAbs))
+  )
+  (and (= w (@bvsize x)) (= wm1 (- (@bvsize x) 1)))
+  (bvsmod x y)
+  (ite (= u (@bv 0 w))
+    u
+    (ite (and nxLt0 nyLt0)
+      u
+      (ite (and xLt0 nyLt0)
+        (bvadd (bvneg u) y)
+        (ite (and nxLt0 yLt0)
+          (bvadd u y)
+          (bvneg u))))))
+
+(define-cond-rule bv-srem-eliminate
+  ((x ?BitVec) (y ?BitVec) (nm1 Int))
+  (def
+    (xLt0 (= (extract nm1 nm1 x) (@bv 1 1)))
+    (yLt0 (= (extract nm1 nm1 y) (@bv 1 1)))
+    (xAbs (ite xLt0 (bvneg x) x))
+    (yAbs (ite yLt0 (bvneg y) y))
+    (u (bvurem xAbs yAbs))
+  )
+  (= nm1 (- (@bvsize x) 1))
+  (bvsrem x y)
+  (ite xLt0 (bvneg u) u))
+
+(define-cond-rule bv-usubo-eliminate
+  ((x ?BitVec) (y ?BitVec) (n Int))
+  (def
+    (s (bvsub (zero_extend 1 x) (zero_extend 1 y)))
+  )
+  (= n (@bvsize x))
+  (bvusubo x y)
+  (= (extract n n s) (@bv 1 1)))
+; Overflow occurs when
+; 1. (N - P) = P
+; 2. (P - N) = N
+(define-cond-rule bv-ssubo-eliminate
+  ((x ?BitVec) (y ?BitVec) (nm1 Int))
+  (def
+    (n (@bvsize x))
+    (xe (extract nm1 nm1 x))
+    (ye (extract nm1 nm1 y))
+    (s (bvsub x y))
+    (se (extract nm1 nm1 s))
+  )
+  (= nm1 (- n 1))
+  (bvssubo x y)
+  (or
+    (and (and (= xe (@bv 1 1)) (= ye (@bv 0 1))) (= se (@bv 0 1)))
+    (and (and (= xe (@bv 0 1)) (= ye (@bv 1 1))) (= se (@bv 1 1)))))
+
+(define-cond-rule bv-nego-eliminate
+  ((x ?BitVec) (n Int))
+  (= n (- (@bvsize x) 1))
+  (bvnego x)
+  (= x (concat (@bv 1 1) (@bv 0 n))))*)
 end
