src/HOL/CVC/cvc5_dsl_rewrites/temp.thy
@@ -1,0 +1,6 @@
+theory temp
+imports Word
+begin
+
+
+end
