src/HOL/SMT_Examples/ExternalProblemChecking/BV_Rewrites_Elimination.thy
@@ -1,13 +1,11 @@
 (*  Title:      HOL/SMT_Examples/SMT_Examples_CVC.thy
     Author:     Hanna Lachnitt, Stanford University
     Author:     Mathias Fleury, University of Freiburg
-
 *)
-theory BV_Rewrites
+
+theory BV_Rewrites_Elimination
   imports HOL.SMT_CVC
 begin
-
-declare[[smt_trace=false,smt_verbose=false]]
 
 
 end
