src/HOL/SMT_Examples/ExternalProblemChecking/UF_BV_Rewrites.thy
@@ -1,0 +1,92 @@
+(*  Title:      HOL/SMT_Examples/SMT_Examples/ExternalProblemChecking/UF_BV_Rewrites.thy
+    Author:     Hanna Lachnitt, Stanford University
+    Author:     Mathias Fleury, University of Freiburg
+*)
+
+theory UF_BV_Rewrites
+    imports HOL.SMT_CVC_Word HOL.Real
+begin
+
+declare[[rare_rec_mode=1]]
+
+declare[[smt_trace=false,smt_verbose=false]]
+
+check_smt_dir ("cvc5_proof") "~~/src/HOL/SMT_Examples/ExternalProblemChecking/Benchmarks/UF_BV_Rewrites/"
+
+declare[[smt_trace=true,smt_verbose=true]]
+
+declare[[smt_expert_debug_alethe_level=3]]
+declare[[smt_expert_debug_alethe_files="alethe_replay_rare"]]
+
+
+(*(define-cond-rule uf-bv2nat-int2bv ((w Int) (t ?BitVec))
+  (= (@bvsize t) w)
+  (int_to_bv w (ubv_to_int t))
+  t)*)
+
+check_smt ("cvc5_proof")
+  "~~/src/HOL/SMT_Examples/ExternalProblemChecking/Benchmarks/UF_Rewrites/uf-bv2nat-int2bv.smt2"
+  "~~/src/HOL/SMT_Examples/ExternalProblemChecking/Benchmarks/UF_Rewrites/uf-bv2nat-int2bv.alethe"
+
+(*(define-cond-rule uf-bv2nat-int2bv-extend ((w Int) (t ?BitVec) (n Int))
+  (and (> w (@bvsize t)) (= n (- w (@bvsize t))))
+  (int_to_bv w (ubv_to_int t))
+  (concat (@bv 0 n) t))*)
+
+check_smt ("cvc5_proof")
+  "~~/src/HOL/SMT_Examples/ExternalProblemChecking/Benchmarks/UF_Rewrites/uf-bv2nat-int2bv-extend.smt2"
+  "~~/src/HOL/SMT_Examples/ExternalProblemChecking/Benchmarks/UF_Rewrites/uf-bv2nat-int2bv-extend.alethe"
+
+(*(define-cond-rule uf-bv2nat-int2bv-extract ((w Int) (t ?BitVec) (wm1 Int))
+  (and (< w (@bvsize t)) (= wm1 (- w 1)))
+  (int_to_bv w (ubv_to_int t))
+  (extract wm1 0 t))*)
+
+check_smt ("cvc5_proof")
+  "~~/src/HOL/SMT_Examples/ExternalProblemChecking/Benchmarks/UF_Rewrites/uf-bv2nat-int2bv-extract.smt2"
+  "~~/src/HOL/SMT_Examples/ExternalProblemChecking/Benchmarks/UF_Rewrites/uf-bv2nat-int2bv-extract.alethe"
+
+(*(define-rule uf-int2bv-bv2nat ((w Int) (t Int))
+  (ubv_to_int (int_to_bv w t))
+  (mod_total t (int.pow2 w)))*)
+
+check_smt ("cvc5_proof")
+  "~~/src/HOL/SMT_Examples/ExternalProblemChecking/Benchmarks/UF_Rewrites/uf-int2bv-bv2nat.smt2"
+  "~~/src/HOL/SMT_Examples/ExternalProblemChecking/Benchmarks/UF_Rewrites/uf-int2bv-bv2nat.alethe"
+
+(*(define-cond-rule uf-bv2nat-geq-elim ((x ?BitVec) (n Int) (w Int))
+  (= w (@bvsize x))
+  (>= (ubv_to_int x) n)
+  (ite (>= n w) false (ite (< n 0) true (bvuge x (int_to_bv w n)))))*)
+
+check_smt ("cvc5_proof")
+  "~~/src/HOL/SMT_Examples/ExternalProblemChecking/Benchmarks/UF_Rewrites/uf-bv2nat-geq-elim.smt2"
+  "~~/src/HOL/SMT_Examples/ExternalProblemChecking/Benchmarks/UF_Rewrites/uf-bv2nat-geq-elim.alethe"
+
+(*(define-rule uf-int2bv-bvult-equiv ((t ?BitVec) (s ?BitVec))
+  (bvult t s)
+  (< (ubv_to_int t) (ubv_to_int s)))*)
+
+check_smt ("cvc5_proof")
+  "~~/src/HOL/SMT_Examples/ExternalProblemChecking/Benchmarks/UF_Rewrites/uf-int2bv-bvult-equiv.smt2"
+  "~~/src/HOL/SMT_Examples/ExternalProblemChecking/Benchmarks/UF_Rewrites/uf-int2bv-bvult-equiv.alethe"
+
+(*(define-rule uf-int2bv-bvule-equiv ((t ?BitVec) (s ?BitVec))
+  (bvule t s)
+  (<= (ubv_to_int t) (ubv_to_int s)))*)
+
+check_smt ("cvc5_proof")
+  "~~/src/HOL/SMT_Examples/ExternalProblemChecking/Benchmarks/UF_Rewrites/uf-int2bv-bvule-equiv.smt2"
+  "~~/src/HOL/SMT_Examples/ExternalProblemChecking/Benchmarks/UF_Rewrites/uf-int2bv-bvule-equiv.alethe"
+
+(*(define-cond-rule uf-sbv-to-int-elim ((t ?BitVec) (wm1 Int) (n Int))
+  (and (= wm1 (- (@bvsize t) 1)) (= n (int.pow2 (@bvsize t))))
+  (sbv_to_int t)
+  (ite (= (extract wm1 wm1 t) (@bv 0 1)) (ubv_to_int t) (- (ubv_to_int t) n)))*)
+
+check_smt ("cvc5_proof")
+  "~~/src/HOL/SMT_Examples/ExternalProblemChecking/Benchmarks/UF_Rewrites/uf-sbv-to-int-elim.smt2"
+  "~~/src/HOL/SMT_Examples/ExternalProblemChecking/Benchmarks/UF_Rewrites/uf-sbv-to-int-elim.alethe"
+
+
+end
