src/HOL/SMT_Examples/ExternalProblemChecking/Benchmarks/UF_BV_Rewrites/bv-not-idemp.smt2
@@ -1,0 +1,6 @@
+(set-logic QF_BV)
+(declare-fun s () (_ BitVec 32))
+(declare-fun t () (_ BitVec 32))
+(assert (not (= (bvnot (bvnot s)) s)))
+(check-sat)
+(exit)
